Prove a version of whole_prog_spec_semantics_prog for ffidiv
In the future, it would be much nicer to have a theorem that supports
programs that can either FFI-diverge or terminate normally.

basis/basis_ffiScript.sml
@@ -335,6 +335,14 @@ val whole_prog_spec_def = Define`
       (POSTv uv. &UNIT_TYPE () uv * STDIO fs') ∧
     post (fs' with numchars := fs.numchars)`;
 
+val whole_prog_ffidiv_spec_def = Define`
+  whole_prog_ffidiv_spec fv cl fs post ⇔
+    ∃fs' n' c' b'.
+    app (basis_proj1, basis_proj2) fv [Conv NONE []]
+      (COMMANDLINE cl * STDIO fs * RUNTIME)
+      (POSTf n. λc b. STDIO fs' * RUNTIME * &(n = n' /\ c = c' /\ b = b')) ∧
+    post n' c' b' (fs' with numchars := fs.numchars)`;
+
 val whole_prog_spec_semantics_prog = Q.store_thm("whole_prog_spec_semantics_prog",
   `∀fname fv.
      ML_code env1 (init_state (basis_ffi cl fs)) prog NONE env2 st2 ==>
@@ -383,6 +391,54 @@ val whole_prog_spec_semantics_prog = Q.store_thm("whole_prog_spec_semantics_prog
   \\ fs[basis_proj1_write,STAR_def,cond_def]
   \\ metis_tac[]
   );
+
+val whole_prog_spec_semantics_prog_ffidiv = Q.store_thm("whole_prog_spec_semantics_prog_ffidiv",
+  `∀fname fv.
+     ML_code env1 (init_state (basis_ffi cl fs)) prog NONE env2 st2 ==>
+     lookup_var fname env2 = SOME fv ==>
+     whole_prog_ffidiv_spec fv cl fs Q ==>
+     (?h1 h2. SPLIT (st2heap (basis_proj1, basis_proj2) st2) (h1,h2) /\ (COMMANDLINE cl * STDIO fs * RUNTIME) h1)
+   ==>
+   ∃io_events fs' n c b.
+     semantics_prog (init_state (basis_ffi cl fs)) env1
+       (SNOC ^main_call prog)
+       (Terminate (FFI_outcome(Final_event n c b FFI_diverged)) io_events) /\
+     extract_fs fs io_events = SOME fs' ∧ Q n c b fs'`,
+  rw[whole_prog_ffidiv_spec_def]
+  \\ drule (GEN_ALL call_main_thm2_ffidiv)
+  \\ rpt(disch_then drule)
+  \\ disch_then (qspecl_then [`basis_proj2`,`basis_proj1`] mp_tac)
+  \\ disch_then (qspecl_then [`h2`, `h1`] mp_tac)
+  \\ disch_then (qspec_then `\n c b. STDIO fs' * RUNTIME * &(n = n' ∧ c = c' ∧ b = b')` mp_tac)
+  \\ disch_then (qspec_then `COMMANDLINE cl * STDIO fs * RUNTIME` mp_tac)
+  \\ simp[] \\ strip_tac
+  \\ asm_exists_tac \\ rw[]
+  \\ rw[extract_fs_def,PULL_EXISTS]
+  \\ drule RTC_call_FFI_rel_IMP_basis_events
+  \\ simp[Once ml_progTheory.init_state_def,Once basis_ffi_def]
+  \\ simp[Once ml_progTheory.init_state_def,Once basis_ffi_def]
+  \\ simp[Once extract_fs_with_numchars_def]
+  \\ simp[Once ml_progTheory.init_state_def]
+  \\ rw[basis_proj1_write,Once basis_ffi_def]
+  \\ `n = n' /\ c = c' /\ b = b'` by(fs[STAR_def,cond_def])
+  \\ rveq
+  \\ `∃ll. SND st3.ffi.ffi_state = fs' with numchars := ll` suffices_by ( rw[] \\ rw[] )
+  \\ fs[STDIO_def, IOFS_def,cfHeapsBaseTheory.IO_def,
+        cfHeapsBaseTheory.IOx_def, set_sepTheory.SEP_CLAUSES,
+        set_sepTheory.SEP_EXISTS_THM, fsFFITheory.fs_ffi_part_def]
+  \\ fs[GSYM set_sepTheory.STAR_ASSOC]
+  \\ fs[Once STAR_def]
+  \\ fs[set_sepTheory.one_STAR]
+  \\ qmatch_assum_abbrev_tac`one ffip _`
+  \\ fs[one_def]
+  \\ `ffip ∈ (st2heap (basis_proj1,basis_proj2) st3)` by cfHeapsBaseLib.SPLIT_TAC
+  \\ fs [cfStoreTheory.st2heap_def, cfStoreTheory.FFI_part_NOT_IN_store2heap,
+         Abbr`ffip`,cfStoreTheory.ffi2heap_def]
+  \\ Cases_on `parts_ok st3.ffi (basis_proj1, basis_proj2)`
+  \\ fs[FLOOKUP_DEF, MAP_MAP_o, n2w_ORD_CHR_w2n, basis_proj1_write]
+  \\ FIRST_X_ASSUM(ASSUME_TAC o Q.SPEC`"write"`)
+  \\ fs[basis_proj1_write,STAR_def,cond_def]
+  \\ metis_tac[]);
 
 val heap_thms = [COMMANDLINE_precond, STDIO_precond];
 
